---
title: Response to Exponential Inputs
subtitle: Exponential
author: Jasper Day
---

# Response to Exponential Input

We start with an equation of form 

$$
\frac{dy}{dt} = ay + e^{st}
$${#eq-source}

The output, $y(t)$, is called the "exponential response."

We have a starting deposit (initial condition) $y = y(0)$ at time $t = 0$, and additional deposits equalling $e^{st}$. 

With @eq-source, the solutions will be a multiple of $e^{st}$, written 

$$
y_p = Ye^{st}
$${#eq-yp}

($y_p$ is a *particular* solution of y.)

So we can substitute @eq-yp into @eq-source and solve for $Y$.

$$
\begin{gathered}
Yse^{st} = aYe^{st} + e^{st} \\
(s-a)Y = 1
Y = \frac{1}{s-a}
\end{gathered}
$$

We've found a particular solution, but to find the complete set of solutions, we need to add all null solutions, where the input is zero.

$$
\begin{gathered}
\frac{dy}{dt} = ay \\
y = e^at
\end{gathered}
$$

So the complete set of solutions $y_p + y_n$ is:

$$
y(t) = \frac{e^{st}}{s-a} + Ce^{at}
$$

and

$$
y(0) = \frac{1}{s-a} + C
$$

The complete solution that satisfies the initial conditions is:

$$
\begin{aligned}
y(t) &= \frac{e^{st}}{s-a} + \left[ y(0) - \frac{1}{s-a} \right]e^{at} \\
&= \frac{e^{st}-e^{at}}{s-a} + y(0)e^{at}
\end{aligned}
$$

$y(0)e^{at}$ is the term growing out of the initial deposit (to use the money-in-the-bank scenario again), and $\frac{e^{st}-e^{at}}{s-a}$ is the term growing out of the additional deposits. 

$\frac{e^{st}-e^{at}}{s-a}$ is the "very particular solution", since it equals $0$ at $t=0$, giving us the form $y_{vp} + y_n$.

## Resonance

There is one problem: what if $s=a$?

Then you have *resonance*: you are putting money in with the same exponential as the natural growth of the money, and our formula has to change. The very particular solution will then be $\frac{0}{0}$: the formula has broken down.

So IF $s=a$,

$$
y_{vp} + y_n = te^{at} + y(0)e^{at}
$${#eq-resonance}

How do we get the resonant answer? We use *l'HÃ´pital's rule*. 

$$
\begin{aligned}
\lim_{s\to a} \frac{e^{st}-e^{at}}{s-a} &= \frac{\frac{d}{ds}\left(e^{st} - e^{at} \right)}{\frac{d}{ds}(s-a)} \\
&= \frac{te^{st}}{1} \\
&= te^{at}
\end{aligned}
$$ {#eq-hopital}

^[Clearly, @eq-hopital works whether you take the derivative with respect to $s$ or with respect to $a$.]

## Sum

So, to recap: 

1. Find a particular solution $y_p$
2. Find the nullspace, all solutions where the input (in this case $e^st$ equals zero)
3. Combine the particular and null solutions, then find an equation in terms of $y(0)$
4. Check for resonance