---
title: Linear Differential Equations
subtitle: Linear constant coefficient homogeneous differential equations
author: Jasper Day
date: 2022/09/20
---

# Introduction to Differential Equations

There are two main types of differential equations: *Ordinary* and *partial*. Partial differential lequations involve partial derivatives of vectors; ordinary differential equations do not. These are simpler to solve than partial DEs.

In $\frac{df}{dx}$, f is the *dependent variable* and x is the *independent variable*.

The *order* of a differential equation is the degree of the highest derivative occuring in that equation.

## Linear vs Nonlinear

*Linear equations* are those equations in which the **dependent variables and their derivatives** do not occur as products, raised to powers or in nonlinear functions. *Nonlinear equations* are all other equations. 

## Homogeneous and Nonhomogeneous

### How to arrange differential equations

The terms with the *dependent variable* go on the left hand side (ie $x$ in $\frac{dx}{dt}$), and all terms not containing the dependent variable (either terms containing only the independent variable, in this case $t$, or constant terms) go on the right hand side of the equation.

### Determining

When the terms are [arranged properly](1_Linear_DE.qmd#how-to-arrange-differential-equations), then **if the right hand side of the equation is ZERO** then the equation is **homogeneous**. If the right hand side (terms without the dependent variable) is **NONZERO**, then the equation is **nonhomogeneous**.

In other words, each term in a homogeneous differential equation involves a dependent variable or its derivatives.

# Solutions to differential equations

The solutions to differential equations generally comprise a function space, or family of related functions.

## 1st order linear differential equations

For the equation
$$
a\frac{dx}{dt} + bx = 0, x \ne 0,
$$

with constant coefficients $a$ and $b$, the general solution is 

$$
x = Ae^{mt}, \textnormal{where } am + b = 0
$$

## Second Order DEs

Now consider what happens with a 2nd order DE:

$$
a\frac{d^2x}{dt^2} + b\frac{dx}{dt} + cx = 0, a \ne 0
$$

Substituting $x(t) = e^{mt}$, you get 

$$
\begin{gather}
am^2e^{mt} + bme^{mt} + ce^{mt} = 0 \\
e^{mt}\left( am^2 + bm + c \right) = 0
\end{gather}
$$

So $x(t) = e^{mt}$ is a solution if $am^2 + bm + c = 0$. 

$am^2 + bm + c = 0$ is the characteristic equation. It's a quadratic; it has 2 roots $m_1$ and $m_2$.

### Distinct real roots

When $m_1$ and $m_2$ are distinct real roots, then 

$x(t) = Ae^{m_1t} + Be^{m_2t}$ (all linear combinations of $e^{m_1t}$ and $e^{m_2t}$.)

### Complex roots

When $m_1$ and $m_2$ are complex conjugates, it's slightly more complex. $m_1 = \phi + j\psi$ and $m_2 = \phi - j\psi$. 

:::{.callout-note}

Here's a quick proof that complex roots must come as conjugates $z = \phi + j\psi$ and 
$z^\star = \phi - j\psi$:

First suppose we have some polynomial $P(x) = a_nx^n + a_{n-1}x^{n-1}+...+a_1x^1+a_0$ such that 
$P(\phi + j\psi) = 0$. The binomial expansion of 
$(\phi + j\psi)^n$ is 

$$
\psi^n + {n \choose 1}j\psi^{n-1}\phi + {n \choose 2}j^2\psi^{n-2}\phi^2 + ... + {n \choose n-1}j^{n-1}\psi\phi^{n-1} + j^n\phi^n.
$$

Only the odd terms of this binomial expansion are imaginary; the even terms are real.

The binomial expansion of $(\phi - j\psi)^n$ is

$$
\psi^n + {n \choose 1}(-j)\psi^{n-1}\phi + {n \choose 2}(-j)^2\psi^{n-2}\phi^2 + ... + {n \choose n-1}(-j)^{n-1}\psi\phi^{n-1} + (-j)   ^n\phi^n.
$$

Comparing the two binomial expansions, the odd terms have switched sign. This means that the imaginary part of the second binomial expansion is the exact negative of the imaginary part of the first binomial expansion; **powers of complex conjugates remain conjugates**.

Since exponentiation and multiplication by a constant preserve conjugacy, $P(z^\star) = P(z)^\star$. Since 
$P(z) = 0$, and 
$0^\star = 0$, 
$P(z^\star) = 0$ for all $P(z) = 0$.

:::

$$
\begin{align}
x(t) &= Ae^{\phi + j\psi t} + Be^{\phi - j\psi t} \\
&= e^{\phi t} \left( Ae^{j\psi t}  + Be^{-j\psi t}\right) \\
&= e^{\phi t}[(A + B)\cos{\psi t} + j(A - B)\cos{\psi t}]
\end{align}
$$

You may further simplify by making $A + B = C$ and $A - B = D$.

### The Same Root

If $m_1 = m_2 = k$, then the general solution with linear superposition breaks down (the function vectors are no longer linearly independent and are not sufficient to span a function space).

For a differential equation to have a repeated root at m = k, then the characteristic quadratic must be a square:

$$
\begin{gather}
am^2 - 2akm + ak^2 = 0 \\
a(m - k)^2 = 0
\end{gather}
$$

Then the differential equation takes this form:

$$
a \frac{d^2x}{dt^2} -2ak \frac{dx}{dt} + ak^2x = 0
$$

Take the "test solution" $x(t) = t^p e^{mt}$. Then $\frac{dx}{dt} = p\left(t^{p-1} \right)e^{mt} + m t^p e^{mt}$ by the power rule and product rule, and 
$$
\frac{d^2x}{dt^2} = m^2 t^p e^{mt} + 2 \left( m p t^{p-1} e^{mt} \right) + p(p-1)t^{p-2}e^mt.
$$

Substitute these expressions into the differential equation:

![](Images/1_Same_Root_DE.png)

For the result to hold, it must be the case that $m = k$ and $p \in \{ 0,1 \}$. Going back to our test solution, we see that either $x(t) = e^{mt}$ or $x(t) = te^{mt}$. Taking the space spanned by these two functions, we find that 

$$
\begin{gather}
x(t) \in \texttt{span}\left(e^{mt}, te^{mt}\right) \\
x(t) = Ae^{mt} + Bte^{mt} \\
x(t) = (A + Bt)e^{mt}
\end{gather}
$$

# Conclusion

To solve a linear homogeneous constant coefficient differential equation, find the roots of the *characteristic equation* with all nth order derivatives replaced with nth powers of x. Then the solutions are the space spanned by all $e^{\textnormal{(root)}t}$, multiplied by a power of $t$ every time a root repeats.
